Trying to automate [msiSv_impl_InvTrs_step]

src/Ex/MsiSvSim.v
@@ -1,8 +1,8 @@
-Require Import Bool List String Peano_dec.
+Require Import Bool List String Peano_dec Omega.
 Require Import Common FMap HVector Syntax Topology Semantics SemFacts StepM.
 Require Import Invariant TrsInv Simulation Serial SerialFacts.
 Require Import RqRsTopo RqRsFacts RqRsLang.
-Require Import RqRsInvLock RqRsMsgPred RqRsCorrect.
+Require Import RqRsInvMsg RqRsInvLock RqRsMsgPred RqRsCorrect.
 
 Require Import Msi MsiSv SpecSv MsiSvTopo.
 
@@ -48,29 +48,27 @@ Definition miisOf (msgs: list (Id Msg)): list Mii :=
   map miiOf msgs.
 
 Definition AtomicMsgOutsInv {oifc} (mp: MsgOutPred oifc)
-           (abf: list Mii -> list Mii)
-           (inits eouts: list (Id Msg)) (nst: MState oifc): Prop :=
-  SubList (miisOf eouts) (abf (miisOf inits)) /\
+           (eouts: list (Id Msg)) (nst: MState oifc): Prop :=
   Forall (fun eout => mp eout nst.(bst_oss)) eouts.
 
 Definition AtomicLocksInv {oifc}
-           (lp: list Mii -> IdxT -> ORq Msg -> Prop)
-           (inits: list (Id Msg)) (hst: MHistory) (nst: MState oifc): Prop :=
+           (lp: IdxT -> ORq Msg -> Prop)
+           (hst: MHistory) (nst: MState oifc): Prop :=
   forall oidx,
     In oidx (oindsOf hst) ->
-    orq <-- (bst_orqs nst)@[oidx]; lp (miisOf inits) oidx orq.
+    orq <-- (bst_orqs nst)@[oidx]; lp oidx orq.
 
 Definition AtomicInv {oifc}
-           (mp: MsgOutPred oifc) (abf: list Mii -> list Mii)
-           (lp: list Mii -> IdxT -> ORq Msg -> Prop):
+           (mp: MsgOutPred oifc)
+           (lp: IdxT -> ORq Msg -> Prop):
   list (Id Msg) (* inits *) ->
   MState oifc (* starting state *) ->
   MHistory (* atomic history *) ->
   list (Id Msg) (* eouts *) ->
   MState oifc (* ending state *) -> Prop :=
   fun inits st1 hst eouts st2 =>
-    AtomicMsgOutsInv mp abf inits eouts st2 /\
-    AtomicLocksInv lp inits hst st2.
+    AtomicMsgOutsInv mp eouts st2 /\
+    AtomicLocksInv lp hst st2.
 
 Section Inv.
 
@@ -109,7 +107,8 @@ Section Inv.
     refine ((oss@[child2Idx]) >>=[False] (fun cost2 => _)).
     refine (post#[implStatusIdx] = msiM /\ _). (* Directory status is M. *)
     exact ((ImplOStateM cv cost1 /\ ImplOStateI cost2) \/
-           (ImplOStateI cost1 /\ ImplOStateM cv cost2)).
+           (ImplOStateI cost1 /\ ImplOStateM cv cost2) \/
+           (ImplOStateS cv cost1 /\ ImplOStateS cv cost2)).
   Defined.
 
   Definition ImplStateCoherent
@@ -120,6 +119,32 @@ Section Inv.
     exists cv, (* The coherent value always exists. *)
       ImplStateCoherent cv st.(bst_oss).
 
+  Ltac disc_msi :=
+    match goal with
+    | [H: ImplStateCoherent _ _ |- _] => red in H
+    | [H: _ \/ _ |- _] => destruct H
+
+    | [H: ImplStateM _ _ |- _] => red in H
+    | [H: ImplStateS _ _ |- _] => red in H
+    | [H: ImplStateI _ |- _] => red in H
+
+    | [H: ImplOStateM _ _ |- _] => destruct H
+    | [H: ImplOStateS _ _ |- _] => destruct H
+    | [H: ImplOStateI _ |- _] => red in H
+
+    | [H: ?oss@[_] = Some ?ost |- _] =>
+      match type of ost with
+      | OState _ =>
+        let val := fresh "val" in
+        let stt := fresh "stt" in
+        destruct ost as [val [stt ?]]
+      end
+    end.
+  
+  Ltac disc_rule_custom ::=
+    try disc_msi;
+    try (unfold msiI, msiS, msiM in *; omega).
+  
   Section Facts.
 
     Lemma implStateCoherent_M_value_changed:
@@ -132,44 +157,30 @@ Section Inv.
           forall n uv,
             ImplStateCoherent n (oss +[oidx <- (n, (msiM, uv))]).
     Proof.
-      intros.
-      destruct H as [|[|]].
-      - exfalso; red in H.
-        disc_rule_conds_ex.
-        destruct H0; subst.
-        + disc_rule_conds_ex.
-          red in H3; simpl in H3.
-          rewrite H3 in H2; discriminate.
-        + disc_rule_conds_ex.
-          red in H4; simpl in H4.
-          rewrite H4 in H2; discriminate.
-      - exfalso; red in H.
-        disc_rule_conds_ex.
-        destruct H0; subst.
-        + disc_rule_conds_ex.
-          destruct H3;
-            try (dest; simpl in H0; rewrite H0 in H2; discriminate).
-        + disc_rule_conds_ex.
-          destruct H4;
-            try (dest; simpl in H0; rewrite H0 in H2; discriminate).
+      intros; solve_rule_conds_ex.
       - right; right.
-        red in H.
-        disc_rule_conds_ex.
-        destruct H0; subst.
-        + destruct H3; dest.
-          * red; red in H0, H3; dest.
-            solve_rule_conds_ex.
-            left; solve_rule_conds_ex.
-          * red; red in H0, H3; dest.
-            solve_rule_conds_ex.
-            left; solve_rule_conds_ex.
-        + destruct H3; dest.
-          * red; red in H0, H3; dest.
-            solve_rule_conds_ex.
-            right; solve_rule_conds_ex.
-          * red; red in H0, H3; dest.
-            solve_rule_conds_ex.
-            right; solve_rule_conds_ex.
+        red; solve_rule_conds_ex.
+        left; solve_rule_conds_ex.
+      - right; right.
+        red; solve_rule_conds_ex.
+        right; left; solve_rule_conds_ex.
+    Qed.
+
+    Lemma implStateCoherent_M_downgraded_to_S:
+      forall cv oss,
+        ImplStateCoherent cv oss ->
+        forall oidx ost,
+          (oidx = child1Idx \/ oidx = child2Idx) ->
+          oss@[oidx] = Some ost ->
+          ost#[implStatusIdx] >= msiS ->
+          ImplStateCoherent cv (oss +[oidx <- (fst ost, (msiS, snd (snd ost)))]).
+    Proof.
+      intros; solve_rule_conds_ex.
+      all: try (right; left; red; solve_rule_conds_ex; auto; fail).
+      all: try (right; right;
+                red; solve_rule_conds_ex;
+                right; right;
+                solve_rule_conds_ex).
     Qed.
 
     Lemma msiSv_impl_InvTrs_ext_in:
@@ -197,19 +208,35 @@ Section Inv.
     Definition MsiSvMsgOutPred: MsgOutPred ImplOStateIfc :=
       fun eout oss =>
         match case (miiOf eout) on mii_dec default True with
+        | (ec1, Spec.getRq): False
+        | (ec1, Spec.setRq): False
+        | (ec1, Spec.evictRq): False
+        | (ec2, Spec.getRq): False
+        | (ec2, Spec.setRq): False
+        | (ec2, Spec.evictRq): False
+                           
+        (* | (pc1, msiDownRqS): *)
+        (*     cost1 <-- oss@[child1Idx]; *)
+        (*     (cost1#[implStatusIdx] = msiM) *)
+        (* | (pc2, msiDownRqS): *)
+        (*     cost2 <-- oss@[child2Idx]; *)
+        (*     (cost2#[implStatusIdx] = msiM) *)
+              
         | (pc1, msiRsS): 
             post <-- oss@[parentIdx];
             cost2 <-- oss@[child2Idx];
             (post#[implStatusIdx] = msiS /\
              cost2#[implStatusIdx] = msiS /\
-             msg_value (valOf eout) = VNat post#[implValueIdx])
+             msg_value (valOf eout) = VNat post#[implValueIdx] /\
+             post#[implValueIdx] = cost2#[implValueIdx])
         | (pc2, msiRsS):
             post <-- oss@[parentIdx];
             cost1 <-- oss@[child1Idx];
             (post#[implStatusIdx] = msiS /\
              cost1#[implStatusIdx] = msiS /\
-             msg_value (valOf eout) = VNat post#[implValueIdx])
-        | (pc1, msiRsM): 
+             msg_value (valOf eout) = VNat post#[implValueIdx] /\
+             post#[implValueIdx] = cost1#[implValueIdx])
+        | (pc1, msiRsM):
             post <-- oss@[parentIdx];
             cost2 <-- oss@[child2Idx];
             (post#[implStatusIdx] = msiM /\ cost2#[implStatusIdx] = msiI)
@@ -243,100 +270,46 @@ Section Inv.
         (** TODO: need a lemma [rsEdgeUpFrom dtr oidx = Some _ -> In oidx (indsOf dtr)] *)
     Admitted.
 
-    Definition msiSvAtomicBoundF (inits: list Mii): list Mii :=
-      match case inits on miis_dec default nil with
-      | [(ec1, Spec.getRq)]:
-          [(ce1, Spec.getRs); (c1pRq, msiRqS); (pc1, msiRsS);
-             (pc2, msiDownRqS); (c2pRs, msiDownRsS)]
-      | [(ec1, Spec.setRq)]:
-          [(ce1, Spec.setRs); (c1pRq, msiRqM); (pc1, msiRsM);
-             (pc2, msiDownRqM); (c2pRs, msiDownRsM)]
-      | [(ec1, Spec.evictRq)]:
-          [(ce1, Spec.evictRs); (c1pRq, msiRqI); (pc1, msiRsI)]
-      | [(ec2, Spec.getRq)]:
-          [(ce2, Spec.getRs); (c2pRq, msiRqS); (pc2, msiRsS);
-             (pc1, msiDownRqS); (c1pRs, msiDownRsS)]
-      | [(ec2, Spec.setRq)]:
-          [(ce2, Spec.setRs); (c2pRq, msiRqM); (pc2, msiRsM);
-             (pc1, msiDownRqM); (c1pRs, msiDownRsM)]
-      | [(ec2, Spec.evictRq)]:
-          [(ce2, Spec.evictRs); (c2pRq, msiRqI); (pc2, msiRsI)]
+    Definition MsiSvLockPred (oidx: IdxT) (orq: ORq Msg): Prop :=
+      match case oidx on eq_nat_dec default True with
+      | child1Idx:
+          rqiu <+- orq@[upRq]; (rqiu.(rqi_midx_rsb) = ce1)
+      | child2Idx:
+          rqiu <+- orq@[upRq]; (rqiu.(rqi_midx_rsb) = ce2)
       end.
 
-    Definition MsiSvLockPred (inits: list Mii) (oidx: IdxT) (orq: ORq Msg): Prop :=
-      match case inits on miis_dec default False with
-      | [(ec1, Spec.getRq)]:
-          match case oidx on eq_nat_dec default True with
-          | child1Idx:
-              rqiu <+- orq@[upRq];
-              (rqiu.(rqi_minds_rss) = [pc1])
-          | parentIdx:
-              rqid <+- orq@[downRq];
-              (rqid.(rqi_minds_rss) = [c2pRs])
-          end
-      | [(ec1, Spec.setRq)]:
-          match case oidx on eq_nat_dec default True with
-          | child1Idx:
-              rqiu <+- orq@[upRq];
-              (rqiu.(rqi_minds_rss) = [pc1])
-          | parentIdx:
-              rqid <+- orq@[downRq];
-              (rqid.(rqi_minds_rss) = [c2pRs])
-          end
-      | [(ec1, Spec.evictRq)]:
-          match case oidx on eq_nat_dec default True with
-          | child1Idx:
-              rqiu <+- orq@[upRq];
-              (rqiu.(rqi_minds_rss) = [pc1])
-          | parentIdx: True
-          end
-      | [(ec2, Spec.getRq)]:
-          match case oidx on eq_nat_dec default True with
-          | child2Idx:
-              rqiu <+- orq@[upRq];
-              (rqiu.(rqi_minds_rss) = [pc2])
-          | parentIdx:
-              rqid <+- orq@[downRq];
-              (rqid.(rqi_minds_rss) = [c1pRs])
-          end
-      | [(ec2, Spec.setRq)]:
-          match case oidx on eq_nat_dec default True with
-          | child2Idx:
-              rqiu <+- orq@[upRq];
-              (rqiu.(rqi_minds_rss) = [pc2])
-          | parentIdx:
-              rqid <+- orq@[downRq];
-              (rqid.(rqi_minds_rss) = [c1pRs])
-          end
-      | [(ec2, Spec.evictRq)]:
-          match case oidx on eq_nat_dec default True with
-          | child2Idx:
-              rqiu <+- orq@[upRq];
-              (rqiu.(rqi_minds_rss) = [pc2])
-          | parentIdx: True
-          end
-      end.
-
-    Ltac disc_rule_custom ::=
+    Ltac disc_AtomicInv :=
       repeat
         match goal with
-        | [H: AtomicInv _ _ _ _ _ _ _ _ |- _] => red in H; dest
-        | [H: AtomicMsgOutsInv _ _ _ _ _ |- _] => red in H; dest
+        | [H: AtomicInv _ _ _ _ _ _ _ |- _] => red in H; dest
         end.
+
+    Ltac disc_rule_custom ::=
+      try disc_footprints_ok;
+      try disc_AtomicInv.
 
     Ltac atomic_cont_exfalso_bound :=
       exfalso;
       disc_rule_conds_ex;
       repeat 
         match goal with
-        | [H1: SubList [_] ?eouts, H2: SubList (miisOf ?eouts) _ |- _] =>
-          let Hs := fresh "H" in
-          pose proof (SubList_trans (SubList_map miiOf H1) H2) as Hs;
-          clear -Hs; apply SubList_singleton_In in Hs; cbn in Hs
-        | [H: context[miis_dec ?miis1 ?miis2] |- _] =>
-          destruct (miis_dec miis1 miis2) in H;
-          try (Common.dest_in; discriminate)
-        end.
+        | [H: SubList [_] ?eouts |- _] => apply SubList_singleton_In in H
+        | [H1: AtomicMsgOutsInv _ ?eouts _, H2: In _ ?eouts |- _] =>
+          red in H1; rewrite Forall_forall in H1;
+          specialize (H1 _ H2); simpl in H1
+        | [H: MsiSvMsgOutPred _ _ |- _] => red in H
+        | [H1: caseDec _ ?mii _ _ |- _] =>
+          match mii with
+          | miiOf (?midx, ?msg) =>
+            match goal with
+            | [H2: msg_id ?msg = ?mid |- _] =>
+              progress replace mii with (midx, mid) in H1
+                by (unfold miiOf; simpl; rewrite H2; reflexivity);
+              simpl in H1
+            end
+          end
+        end;
+      assumption.
 
     Ltac atomic_init_exfalso_rq :=
       exfalso;
@@ -382,23 +355,8 @@ Section Inv.
         apply SubList_singleton_In in H1; dest_in
       end.
 
-    Ltac atomic_init_solve_AtomicMsgOutsInv_subList :=
-      simpl; unfold miiOf; simpl;
-      repeat
-        match goal with
-        | [H: msg_id ?msg = _ |- context [msg_id ?msg] ] => rewrite H
-        | [H1: msg_id ?msg = _, H2: context [msg_id ?msg] |- _] =>
-          rewrite H1 in H2
-        end;
-      repeat
-        match goal with
-        | [ |- SubList [_] _] => apply SubList_cons; [|apply SubList_nil]
-        | [ |- In _ _] => simpl; tauto
-        end.
-
     Ltac atomic_init_solve_AtomicMsgOutsInv :=
-      split; [atomic_init_solve_AtomicMsgOutsInv_subList|
-              simpl; repeat constructor].
+      simpl; repeat constructor.
 
     Ltac atomic_init_solve_AtomicLocksInv :=
       red; intros; dest_in;
@@ -416,11 +374,11 @@ Section Inv.
         | [H1: ?orq@[?i] = None, H2: context [?orq@[?i]] |- _] =>
           rewrite H1 in H2
         end;
-      red; simpl; mred.
+      repeat (red; simpl; mred; auto).
 
     Local Ltac atomic_init_solve_AtomicInv :=
-      split; [atomic_init_solve_AtomicMsgOutsInv|
-              atomic_init_solve_AtomicLocksInv].
+      split; [atomic_init_solve_AtomicMsgOutsInv
+             |atomic_init_solve_AtomicLocksInv].
 
     Lemma msiSv_impl_InvTrs_init:
       forall st1,
@@ -429,8 +387,9 @@ Section Inv.
         forall oidx ridx ins outs st2,
           SubList (idsOf ins) (sys_merqs impl) ->
           step_m impl st1 (RlblInt oidx ridx ins outs) st2 ->
-          AtomicInv MsiSvMsgOutPred msiSvAtomicBoundF MsiSvLockPred
-                    ins st1 [RlblInt oidx ridx ins outs] outs st2 /\
+          AtomicInv
+            MsiSvMsgOutPred MsiSvLockPred
+            ins st1 [RlblInt oidx ridx ins outs] outs st2 /\
           ImplStateMSI st2.
     Proof.
       intros.
@@ -513,69 +472,152 @@ Section Inv.
           solve_midx_false.
     Qed.
 
+    Lemma miisOf_app:
+      forall miis1 miis2,
+        miisOf (miis1 ++ miis2) = miisOf miis1 ++ miisOf miis2.
+    Proof.
+      unfold miisOf; intros.
+      apply map_app.
+    Qed.
+
+    Ltac disc_minds_const :=
+      repeat
+        match goal with
+        | [H: rqEdgeUpFrom ?dtr ?oidx = Some ?midx |- _] =>
+          is_const dtr; is_const oidx; is_var midx; inv H
+        | [H: rsEdgeUpFrom ?dtr ?oidx = Some ?midx |- _] =>
+          is_const dtr; is_const oidx; is_var midx; inv H
+        | [H: edgeDownTo ?dtr ?oidx = Some ?midx |- _] =>
+          is_const dtr; is_const oidx; is_var midx; inv H
+        end.
+
+    Ltac disc_rule_custom ::=
+      try disc_footprints_ok;
+      try disc_AtomicInv;
+      try disc_minds_const.
+
+    Opaque upRq downRq.
+
     Lemma msiSv_impl_InvTrs: InvTrs impl ImplStateMSI.
     Proof.
       eapply inv_atomic_InvTrs;
         [red; intros; eapply msiSv_impl_InvTrs_ext_in; eauto
         |red; intros; eapply msiSv_impl_InvTrs_ext_out; eauto
         |].
-      instantiate (1:= AtomicInv
-                         MsiSvMsgOutPred
-                         msiSvAtomicBoundF
-                         MsiSvLockPred).
-
+      instantiate (1:= AtomicInv MsiSvMsgOutPred MsiSvLockPred).
       red; intros.
       destruct H1.
       generalize dependent ist2.
-      induction H3; simpl; intros; subst.
-      
-      - inv_steps.
-        apply msiSv_impl_InvTrs_init; auto.
+      induction H3; simpl; intros; subst;
+        [inv_steps; apply msiSv_impl_InvTrs_init; auto|].
+
+      inv_steps.
+      pose proof (footprints_ok msiSv_impl_GoodRqRsSys (reachable_steps H H9))
+        as Hftinv.
+      specialize (IHAtomic H1 _ H9); dest.
+      inv_step; dest_in.
+
+      (** child1 *)
+
+      - atomic_cont_exfalso_bound.
+      - atomic_cont_exfalso_bound.
+
+      - (* [childGetRsS] *)
+        disc_rule_conds_ex.
+        good_footprint_get child1Idx.
+        disc_rule_conds_ex.
+
+        apply SubList_singleton_In in H4.
+        pose proof H7.
+        red in H21; simpl in H21.
+        assert (In child1Idx (oindsOf hst)).
+        { eapply extAtomic_rsDown_acceptor_visited; eauto.
+          { exact msiSv_impl_RqRsSys. }
+          { econstructor; eassumption. }
+          { red; auto. }
+        }
+        specialize (H21 _ H22); clear H22.
+        disc_rule_conds_ex.
+
+        red in H21; simpl in H21.
+        disc_rule_conds_ex.
+
+        red in H5; rewrite Forall_forall in H5.
+        specialize (H5 _ H4); simpl in H5.
+        red in H5.
+        match goal with
+        | [H1: caseDec _ ?mii _ _ |- _] =>
+          match mii with
+          | miiOf (?midx, ?msg) =>
+            match goal with
+            | [H2: msg_id ?msg = ?mid |- _] =>
+              progress replace mii with (midx, mid) in H1
+                by (unfold miiOf; simpl; rewrite H2; reflexivity);
+                simpl in H1
+            end
+          end
+        end.
+        disc_rule_conds_ex.
+
+        (* construction *)
         
-      - inv_steps.
-        specialize (IHAtomic H1 _ H9); dest.
-        inv_step; dest_in.
+        split.
+        + split.
+          * match goal with
+            | [ |- AtomicMsgOutsInv _ (?rl ++ _) _ ] =>
+              replace rl with (@nil (Id Msg)) by admit
+            end.
+            repeat (constructor; simpl).
+          * red; simpl; intros.
+            destruct (eq_nat_dec oidx child1Idx);
+              [subst; clear H28
+              |destruct H28; [exfalso; auto|]].
+            { repeat (simpl; red; mred). }
+            { mred; apply H7; auto. }
 
-        (** child1 *)
+        + red; simpl.
+          eexists.
+          right; left.
+          red; solve_rule_conds_ex.
+          * eauto.
+          * right; split; eauto.
+            congruence.
+        
+      - admit.
+      - atomic_cont_exfalso_bound.
+      - atomic_cont_exfalso_bound.
+      - admit.
+      - admit.
+      - atomic_cont_exfalso_bound.
+      - admit.
 
-        + atomic_cont_exfalso_bound.
-        + atomic_cont_exfalso_bound.
-        + admit.
-        + admit.
-        + atomic_cont_exfalso_bound.
-        + atomic_cont_exfalso_bound.
-        + admit.
-        + admit.
-        + atomic_cont_exfalso_bound.
-        + admit.
+      (** child2 *)
 
-        (* child2 *)
+      - atomic_cont_exfalso_bound.
+      - atomic_cont_exfalso_bound.
+      - admit.
+      - admit.
+      - atomic_cont_exfalso_bound.
+      - atomic_cont_exfalso_bound.
+      - admit.
+      - admit.
+      - atomic_cont_exfalso_bound.
+      - admit.
 
-        + atomic_cont_exfalso_bound.
-        + atomic_cont_exfalso_bound.
-        + admit.
-        + admit.
-        + atomic_cont_exfalso_bound.
-        + atomic_cont_exfalso_bound.
-        + admit.
-        + admit.
-        + atomic_cont_exfalso_bound.
-        + admit.
+      (** parent *)
 
-        (* parent *)
-
-        + admit.
-        + admit.
-        + admit.
-        + admit.
-        + admit.
-        + admit.
-        + admit.
-        + admit.
-        + admit.
-        + admit.
-        + admit.
-        + admit.
+      - admit.
+      - admit.
+      - admit.
+      - admit.
+      - admit.
+      - admit.
+      - admit.
+      - admit.
+      - admit.
+      - admit.
+      - admit.
+      - admit.
         
     Admitted.
 
